a version without abstract types/functions

verified_cogent_driver/generated/driver.c
@@ -11,257 +11,257 @@ static inline void d4_set_timer_e(t3 *b, u32 v)
 {
     d5_set_timer_e_part0(b, (unsigned int) (v >> 0U & 4294967295U));
 }
-static inline unsigned int d8_get_timer_e_hi_part0(t3 *b)
-{
-    return (*b).data[19U] >> 0U & 0XFFFFFFFFU;
-}
-static inline u32 d7_get_timer_e_hi(t3 *b)
-{
-    return (u32) d8_get_timer_e_hi_part0(b) << 0U;
-}
-static inline unsigned int d10_get_timer_e_part0(t3 *b)
-{
-    return (*b).data[18U] >> 0U & 0XFFFFFFFFU;
-}
-static inline u32 d9_get_timer_e(t3 *b)
-{
-    return (u32) d10_get_timer_e_part0(b) << 0U;
-}
-static inline void d14_set_timer_a_input_clk_tag_part0(t3 *b, unsigned int v)
-{
-    (*b).data[0U] = ((*b).data[0U] & ~(0X3U << 8U)) | (0X3U & v) << 8U;
-}
-static inline void d13_set_timer_a_input_clk_tag(t3 *b, unsigned int v)
-{
-    d14_set_timer_a_input_clk_tag_part0(b, (unsigned int) (v >> 0U & 3U));
-}
-static inline void d15_set_timer_a_input_clk_TIMEOUT_TIMEBASE_100_US(t3 *b,
-                                                                     unit_t v)
-{ }
-static inline void d16_set_timer_a_input_clk_TIMEOUT_TIMEBASE_10_US(t3 *b,
-                                                                    unit_t v)
-{ }
-static inline void d17_set_timer_a_input_clk_TIMEOUT_TIMEBASE_1_MS(t3 *b,
-                                                                   unit_t v)
-{ }
-static inline void d18_set_timer_a_input_clk_TIMEOUT_TIMEBASE_1_US(t3 *b,
-                                                                   unit_t v)
-{ }
-static inline void d12_set_timer_a_input_clk(t3 *b, t1 v)
-{
-    if (v.tag == TAG_ENUM_TIMEOUT_TIMEBASE_1_US) {
-        d13_set_timer_a_input_clk_tag(b, 0U);
-        d18_set_timer_a_input_clk_TIMEOUT_TIMEBASE_1_US(b,
-                                                        v.TIMEOUT_TIMEBASE_1_US);
-    } else if (v.tag == TAG_ENUM_TIMEOUT_TIMEBASE_1_MS) {
-        d13_set_timer_a_input_clk_tag(b, 3U);
-        d17_set_timer_a_input_clk_TIMEOUT_TIMEBASE_1_MS(b,
-                                                        v.TIMEOUT_TIMEBASE_1_MS);
-    } else if (v.tag == TAG_ENUM_TIMEOUT_TIMEBASE_10_US) {
-        d13_set_timer_a_input_clk_tag(b, 1U);
-        d16_set_timer_a_input_clk_TIMEOUT_TIMEBASE_10_US(b,
-                                                         v.TIMEOUT_TIMEBASE_10_US);
-    } else {
-        d13_set_timer_a_input_clk_tag(b, 2U);
-        d15_set_timer_a_input_clk_TIMEOUT_TIMEBASE_100_US(b,
-                                                          v.TIMEOUT_TIMEBASE_100_US);
-    }
-}
-static inline void d21_set_timer_e_input_clk_tag_part0(t3 *b, unsigned int v)
-{
-    (*b).data[0U] = ((*b).data[0U] & ~(0X7U << 0U)) | (0X7U & v) << 0U;
-}
-static inline void d20_set_timer_e_input_clk_tag(t3 *b, unsigned int v)
-{
-    d21_set_timer_e_input_clk_tag_part0(b, (unsigned int) (v >> 0U & 7U));
-}
-static inline void d22_set_timer_e_input_clk_TIMESTAMP_TIMEBASE_100_US(t3 *b,
-                                                                       unit_t v)
-{ }
-static inline void d23_set_timer_e_input_clk_TIMESTAMP_TIMEBASE_10_US(t3 *b,
-                                                                      unit_t v)
-{ }
-static inline void d24_set_timer_e_input_clk_TIMESTAMP_TIMEBASE_1_MS(t3 *b,
-                                                                     unit_t v)
-{ }
-static inline void d25_set_timer_e_input_clk_TIMESTAMP_TIMEBASE_1_US(t3 *b,
-                                                                     unit_t v)
-{ }
-static inline void d26_set_timer_e_input_clk_TIMESTAMP_TIMEBASE_SYSTEM(t3 *b,
-                                                                       unit_t v)
-{ }
-static inline void d19_set_timer_e_input_clk(t3 *b, t2 v)
-{
-    if (v.tag == TAG_ENUM_TIMESTAMP_TIMEBASE_SYSTEM) {
-        d20_set_timer_e_input_clk_tag(b, 0U);
-        d26_set_timer_e_input_clk_TIMESTAMP_TIMEBASE_SYSTEM(b,
-                                                            v.TIMESTAMP_TIMEBASE_SYSTEM);
-    } else if (v.tag == TAG_ENUM_TIMESTAMP_TIMEBASE_1_US) {
-        d20_set_timer_e_input_clk_tag(b, 1U);
-        d25_set_timer_e_input_clk_TIMESTAMP_TIMEBASE_1_US(b,
-                                                          v.TIMESTAMP_TIMEBASE_1_US);
-    } else if (v.tag == TAG_ENUM_TIMESTAMP_TIMEBASE_1_MS) {
-        d20_set_timer_e_input_clk_tag(b, 4U);
-        d24_set_timer_e_input_clk_TIMESTAMP_TIMEBASE_1_MS(b,
-                                                          v.TIMESTAMP_TIMEBASE_1_MS);
-    } else if (v.tag == TAG_ENUM_TIMESTAMP_TIMEBASE_10_US) {
-        d20_set_timer_e_input_clk_tag(b, 2U);
-        d23_set_timer_e_input_clk_TIMESTAMP_TIMEBASE_10_US(b,
-                                                           v.TIMESTAMP_TIMEBASE_10_US);
-    } else {
-        d20_set_timer_e_input_clk_tag(b, 3U);
-        d22_set_timer_e_input_clk_TIMESTAMP_TIMEBASE_100_US(b,
-                                                            v.TIMESTAMP_TIMEBASE_100_US);
-    }
-}
-static inline void d29_set_timer_a_mode_part0(t3 *b, unsigned int v)
-{
-    (*b).data[0U] = ((*b).data[0U] & ~(0X1U << 11U)) | (0X1U & v) << 11U;
-}
-static inline void d28_set_timer_a_mode(t3 *b, bool_t v)
-{
-    d29_set_timer_a_mode_part0(b, (unsigned int) (v.boolean >> 0U & 1U));
-}
-static inline void d31_set_timer_a_part0(t3 *b, unsigned int v)
-{
-    (*b).data[1U] = ((*b).data[1U] & ~(0XFFFFFFFFU << 0U)) | (0XFFFFFFFFU &
-                                                              v) << 0U;
-}
-static inline void d30_set_timer_a(t3 *b, u32 v)
-{
-    d31_set_timer_a_part0(b, (unsigned int) (v >> 0U & 4294967295U));
-}
-static inline void d33_set_timer_a_en_part0(t3 *b, unsigned int v)
-{
-    (*b).data[0U] = ((*b).data[0U] & ~(0X1U << 15U)) | (0X1U & v) << 15U;
-}
-static inline void d32_set_timer_a_en(t3 *b, bool_t v)
-{
-    d33_set_timer_a_en_part0(b, (unsigned int) (v.boolean >> 0U & 1U));
-}
-static inline unsigned int d35_get_timer_a_en_part0(t3 *b)
-{
-    return (*b).data[0U] >> 15U & 0X1U;
-}
-static inline bool_t d34_get_timer_a_en(t3 *b)
-{
-    return (bool_t) {.boolean = (unsigned char) d35_get_timer_a_en_part0(b) <<
-                     0U};
-}
-static inline unsigned int d37_get_timer_a_part0(t3 *b)
-{
-    return (*b).data[1U] >> 0U & 0XFFFFFFFFU;
-}
-static inline u32 d36_get_timer_a(t3 *b)
-{
-    return (u32) d37_get_timer_a_part0(b) << 0U;
-}
-static inline unsigned int d39_get_timer_a_mode_part0(t3 *b)
-{
-    return (*b).data[0U] >> 11U & 0X1U;
-}
-static inline bool_t d38_get_timer_a_mode(t3 *b)
-{
-    return (bool_t) {.boolean = (unsigned char) d39_get_timer_a_mode_part0(b) <<
-                     0U};
-}
-static inline unsigned int d42_get_timer_a_input_clk_tag_part0(t3 *b)
-{
-    return (*b).data[0U] >> 8U & 0X3U;
-}
-static inline unsigned int d41_get_timer_a_input_clk_tag(t3 *b)
-{
-    return (unsigned int) d42_get_timer_a_input_clk_tag_part0(b) << 0U;
-}
-static inline unit_t d43_get_timer_a_input_clk_TIMEOUT_TIMEBASE_100_US(t3 *b)
-{
-    return (unit_t) {.dummy = 0};
-}
-static inline unit_t d44_get_timer_a_input_clk_TIMEOUT_TIMEBASE_10_US(t3 *b)
-{
-    return (unit_t) {.dummy = 0};
-}
-static inline unit_t d45_get_timer_a_input_clk_TIMEOUT_TIMEBASE_1_MS(t3 *b)
-{
-    return (unit_t) {.dummy = 0};
-}
-static inline unit_t d46_get_timer_a_input_clk_TIMEOUT_TIMEBASE_1_US(t3 *b)
-{
-    return (unit_t) {.dummy = 0};
-}
-static inline t1 d40_get_timer_a_input_clk(t3 *b)
-{
-    return d41_get_timer_a_input_clk_tag(b) == 0U ? (t1) {.tag =
-                                                          TAG_ENUM_TIMEOUT_TIMEBASE_1_US,
-                                                          .TIMEOUT_TIMEBASE_1_US =
-                                                          d46_get_timer_a_input_clk_TIMEOUT_TIMEBASE_1_US(b)} : d41_get_timer_a_input_clk_tag(b) ==
-        3U ? (t1) {.tag = TAG_ENUM_TIMEOUT_TIMEBASE_1_MS,
-                   .TIMEOUT_TIMEBASE_1_MS =
-                   d45_get_timer_a_input_clk_TIMEOUT_TIMEBASE_1_MS(b)} : d41_get_timer_a_input_clk_tag(b) ==
-        1U ? (t1) {.tag = TAG_ENUM_TIMEOUT_TIMEBASE_10_US,
-                   .TIMEOUT_TIMEBASE_10_US =
-                   d44_get_timer_a_input_clk_TIMEOUT_TIMEBASE_10_US(b)} : (t1) {.tag =
-                                                                                TAG_ENUM_TIMEOUT_TIMEBASE_100_US,
-                                                                                .TIMEOUT_TIMEBASE_100_US =
-                                                                                d43_get_timer_a_input_clk_TIMEOUT_TIMEBASE_100_US(b)};
-}
-static inline unsigned int d49_get_timer_e_input_clk_tag_part0(t3 *b)
-{
-    return (*b).data[0U] >> 0U & 0X7U;
-}
-static inline unsigned int d48_get_timer_e_input_clk_tag(t3 *b)
-{
-    return (unsigned int) d49_get_timer_e_input_clk_tag_part0(b) << 0U;
-}
-static inline unit_t d50_get_timer_e_input_clk_TIMESTAMP_TIMEBASE_100_US(t3 *b)
-{
-    return (unit_t) {.dummy = 0};
-}
-static inline unit_t d51_get_timer_e_input_clk_TIMESTAMP_TIMEBASE_10_US(t3 *b)
-{
-    return (unit_t) {.dummy = 0};
-}
-static inline unit_t d52_get_timer_e_input_clk_TIMESTAMP_TIMEBASE_1_MS(t3 *b)
-{
-    return (unit_t) {.dummy = 0};
-}
-static inline unit_t d53_get_timer_e_input_clk_TIMESTAMP_TIMEBASE_1_US(t3 *b)
-{
-    return (unit_t) {.dummy = 0};
-}
-static inline unit_t d54_get_timer_e_input_clk_TIMESTAMP_TIMEBASE_SYSTEM(t3 *b)
-{
-    return (unit_t) {.dummy = 0};
-}
-static inline t2 d47_get_timer_e_input_clk(t3 *b)
-{
-    return d48_get_timer_e_input_clk_tag(b) == 0U ? (t2) {.tag =
-                                                          TAG_ENUM_TIMESTAMP_TIMEBASE_SYSTEM,
-                                                          .TIMESTAMP_TIMEBASE_SYSTEM =
-                                                          d54_get_timer_e_input_clk_TIMESTAMP_TIMEBASE_SYSTEM(b)} : d48_get_timer_e_input_clk_tag(b) ==
-        1U ? (t2) {.tag = TAG_ENUM_TIMESTAMP_TIMEBASE_1_US,
-                   .TIMESTAMP_TIMEBASE_1_US =
-                   d53_get_timer_e_input_clk_TIMESTAMP_TIMEBASE_1_US(b)} : d48_get_timer_e_input_clk_tag(b) ==
-        4U ? (t2) {.tag = TAG_ENUM_TIMESTAMP_TIMEBASE_1_MS,
-                   .TIMESTAMP_TIMEBASE_1_MS =
-                   d52_get_timer_e_input_clk_TIMESTAMP_TIMEBASE_1_MS(b)} : d48_get_timer_e_input_clk_tag(b) ==
-        2U ? (t2) {.tag = TAG_ENUM_TIMESTAMP_TIMEBASE_10_US,
-                   .TIMESTAMP_TIMEBASE_10_US =
-                   d51_get_timer_e_input_clk_TIMESTAMP_TIMEBASE_10_US(b)} : (t2) {.tag =
-                                                                                  TAG_ENUM_TIMESTAMP_TIMEBASE_100_US,
-                                                                                  .TIMESTAMP_TIMEBASE_100_US =
-                                                                                  d50_get_timer_e_input_clk_TIMESTAMP_TIMEBASE_100_US(b)};
-}
-static inline void d56_set_timer_e_hi_part0(t3 *b, unsigned int v)
+static inline void d7_set_timer_e_hi_part0(t3 *b, unsigned int v)
 {
     (*b).data[19U] = ((*b).data[19U] & ~(0XFFFFFFFFU << 0U)) | (0XFFFFFFFFU &
                                                                 v) << 0U;
 }
-static inline void d55_set_timer_e_hi(t3 *b, u32 v)
+static inline void d6_set_timer_e_hi(t3 *b, u32 v)
 {
-    d56_set_timer_e_hi_part0(b, (unsigned int) (v >> 0U & 4294967295U));
+    d7_set_timer_e_hi_part0(b, (unsigned int) (v >> 0U & 4294967295U));
 }
-static inline t3 *reset_timer_e_cogent(t3 *a1)
+static inline void d11_set_timer_a_input_clk_tag_part0(t3 *b, unsigned int v)
+{
+    (*b).data[0U] = ((*b).data[0U] & ~(0X3U << 0U)) | (0X3U & v) << 0U;
+}
+static inline void d10_set_timer_a_input_clk_tag(t3 *b, unsigned int v)
+{
+    d11_set_timer_a_input_clk_tag_part0(b, (unsigned int) (v >> 0U & 3U));
+}
+static inline void d12_set_timer_a_input_clk_TIMEOUT_TIMEBASE_100_US(t3 *b,
+                                                                     unit_t v)
+{ }
+static inline void d13_set_timer_a_input_clk_TIMEOUT_TIMEBASE_10_US(t3 *b,
+                                                                    unit_t v)
+{ }
+static inline void d14_set_timer_a_input_clk_TIMEOUT_TIMEBASE_1_MS(t3 *b,
+                                                                   unit_t v)
+{ }
+static inline void d15_set_timer_a_input_clk_TIMEOUT_TIMEBASE_1_US(t3 *b,
+                                                                   unit_t v)
+{ }
+static inline void d9_set_timer_a_input_clk(t3 *b, t1 v)
+{
+    if (v.tag == TAG_ENUM_TIMEOUT_TIMEBASE_1_US) {
+        d10_set_timer_a_input_clk_tag(b, 0U);
+        d15_set_timer_a_input_clk_TIMEOUT_TIMEBASE_1_US(b,
+                                                        v.TIMEOUT_TIMEBASE_1_US);
+    } else if (v.tag == TAG_ENUM_TIMEOUT_TIMEBASE_1_MS) {
+        d10_set_timer_a_input_clk_tag(b, 3U);
+        d14_set_timer_a_input_clk_TIMEOUT_TIMEBASE_1_MS(b,
+                                                        v.TIMEOUT_TIMEBASE_1_MS);
+    } else if (v.tag == TAG_ENUM_TIMEOUT_TIMEBASE_10_US) {
+        d10_set_timer_a_input_clk_tag(b, 1U);
+        d13_set_timer_a_input_clk_TIMEOUT_TIMEBASE_10_US(b,
+                                                         v.TIMEOUT_TIMEBASE_10_US);
+    } else {
+        d10_set_timer_a_input_clk_tag(b, 2U);
+        d12_set_timer_a_input_clk_TIMEOUT_TIMEBASE_100_US(b,
+                                                          v.TIMEOUT_TIMEBASE_100_US);
+    }
+}
+static inline void d18_set_timer_e_input_clk_tag_part0(t3 *b, unsigned int v)
+{
+    (*b).data[0U] = ((*b).data[0U] & ~(0X7U << 8U)) | (0X7U & v) << 8U;
+}
+static inline void d17_set_timer_e_input_clk_tag(t3 *b, unsigned int v)
+{
+    d18_set_timer_e_input_clk_tag_part0(b, (unsigned int) (v >> 0U & 7U));
+}
+static inline void d19_set_timer_e_input_clk_TIMESTAMP_TIMEBASE_100_US(t3 *b,
+                                                                       unit_t v)
+{ }
+static inline void d20_set_timer_e_input_clk_TIMESTAMP_TIMEBASE_10_US(t3 *b,
+                                                                      unit_t v)
+{ }
+static inline void d21_set_timer_e_input_clk_TIMESTAMP_TIMEBASE_1_MS(t3 *b,
+                                                                     unit_t v)
+{ }
+static inline void d22_set_timer_e_input_clk_TIMESTAMP_TIMEBASE_1_US(t3 *b,
+                                                                     unit_t v)
+{ }
+static inline void d23_set_timer_e_input_clk_TIMESTAMP_TIMEBASE_SYSTEM(t3 *b,
+                                                                       unit_t v)
+{ }
+static inline void d16_set_timer_e_input_clk(t3 *b, t2 v)
+{
+    if (v.tag == TAG_ENUM_TIMESTAMP_TIMEBASE_SYSTEM) {
+        d17_set_timer_e_input_clk_tag(b, 0U);
+        d23_set_timer_e_input_clk_TIMESTAMP_TIMEBASE_SYSTEM(b,
+                                                            v.TIMESTAMP_TIMEBASE_SYSTEM);
+    } else if (v.tag == TAG_ENUM_TIMESTAMP_TIMEBASE_1_US) {
+        d17_set_timer_e_input_clk_tag(b, 1U);
+        d22_set_timer_e_input_clk_TIMESTAMP_TIMEBASE_1_US(b,
+                                                          v.TIMESTAMP_TIMEBASE_1_US);
+    } else if (v.tag == TAG_ENUM_TIMESTAMP_TIMEBASE_1_MS) {
+        d17_set_timer_e_input_clk_tag(b, 4U);
+        d21_set_timer_e_input_clk_TIMESTAMP_TIMEBASE_1_MS(b,
+                                                          v.TIMESTAMP_TIMEBASE_1_MS);
+    } else if (v.tag == TAG_ENUM_TIMESTAMP_TIMEBASE_10_US) {
+        d17_set_timer_e_input_clk_tag(b, 2U);
+        d20_set_timer_e_input_clk_TIMESTAMP_TIMEBASE_10_US(b,
+                                                           v.TIMESTAMP_TIMEBASE_10_US);
+    } else {
+        d17_set_timer_e_input_clk_tag(b, 3U);
+        d19_set_timer_e_input_clk_TIMESTAMP_TIMEBASE_100_US(b,
+                                                            v.TIMESTAMP_TIMEBASE_100_US);
+    }
+}
+static inline unsigned int d25_get_timer_e_hi_part0(t3 *b)
+{
+    return (*b).data[19U] >> 0U & 0XFFFFFFFFU;
+}
+static inline u32 d24_get_timer_e_hi(t3 *b)
+{
+    return (u32) d25_get_timer_e_hi_part0(b) << 0U;
+}
+static inline unsigned int d27_get_timer_e_part0(t3 *b)
+{
+    return (*b).data[18U] >> 0U & 0XFFFFFFFFU;
+}
+static inline u32 d26_get_timer_e(t3 *b)
+{
+    return (u32) d27_get_timer_e_part0(b) << 0U;
+}
+static inline void d30_set_timer_a_mode_part0(t3 *b, unsigned int v)
+{
+    (*b).data[0U] = ((*b).data[0U] & ~(0X1U << 11U)) | (0X1U & v) << 11U;
+}
+static inline void d29_set_timer_a_mode(t3 *b, bool_t v)
+{
+    d30_set_timer_a_mode_part0(b, (unsigned int) (v.boolean >> 0U & 1U));
+}
+static inline void d32_set_timer_a_part0(t3 *b, unsigned int v)
+{
+    (*b).data[1U] = ((*b).data[1U] & ~(0XFFFFFFFFU << 0U)) | (0XFFFFFFFFU &
+                                                              v) << 0U;
+}
+static inline void d31_set_timer_a(t3 *b, u32 v)
+{
+    d32_set_timer_a_part0(b, (unsigned int) (v >> 0U & 4294967295U));
+}
+static inline void d34_set_timer_a_en_part0(t3 *b, unsigned int v)
+{
+    (*b).data[0U] = ((*b).data[0U] & ~(0X1U << 15U)) | (0X1U & v) << 15U;
+}
+static inline void d33_set_timer_a_en(t3 *b, bool_t v)
+{
+    d34_set_timer_a_en_part0(b, (unsigned int) (v.boolean >> 0U & 1U));
+}
+static inline unsigned int d36_get_timer_a_en_part0(t3 *b)
+{
+    return (*b).data[0U] >> 15U & 0X1U;
+}
+static inline bool_t d35_get_timer_a_en(t3 *b)
+{
+    return (bool_t) {.boolean = (unsigned char) d36_get_timer_a_en_part0(b) <<
+                     0U};
+}
+static inline unsigned int d38_get_timer_a_part0(t3 *b)
+{
+    return (*b).data[1U] >> 0U & 0XFFFFFFFFU;
+}
+static inline u32 d37_get_timer_a(t3 *b)
+{
+    return (u32) d38_get_timer_a_part0(b) << 0U;
+}
+static inline unsigned int d40_get_timer_a_mode_part0(t3 *b)
+{
+    return (*b).data[0U] >> 11U & 0X1U;
+}
+static inline bool_t d39_get_timer_a_mode(t3 *b)
+{
+    return (bool_t) {.boolean = (unsigned char) d40_get_timer_a_mode_part0(b) <<
+                     0U};
+}
+static inline unsigned int d43_get_timer_a_input_clk_tag_part0(t3 *b)
+{
+    return (*b).data[0U] >> 0U & 0X3U;
+}
+static inline unsigned int d42_get_timer_a_input_clk_tag(t3 *b)
+{
+    return (unsigned int) d43_get_timer_a_input_clk_tag_part0(b) << 0U;
+}
+static inline unit_t d44_get_timer_a_input_clk_TIMEOUT_TIMEBASE_100_US(t3 *b)
+{
+    return (unit_t) {.dummy = 0};
+}
+static inline unit_t d45_get_timer_a_input_clk_TIMEOUT_TIMEBASE_10_US(t3 *b)
+{
+    return (unit_t) {.dummy = 0};
+}
+static inline unit_t d46_get_timer_a_input_clk_TIMEOUT_TIMEBASE_1_MS(t3 *b)
+{
+    return (unit_t) {.dummy = 0};
+}
+static inline unit_t d47_get_timer_a_input_clk_TIMEOUT_TIMEBASE_1_US(t3 *b)
+{
+    return (unit_t) {.dummy = 0};
+}
+static inline t1 d41_get_timer_a_input_clk(t3 *b)
+{
+    return d42_get_timer_a_input_clk_tag(b) == 0U ? (t1) {.tag =
+                                                          TAG_ENUM_TIMEOUT_TIMEBASE_1_US,
+                                                          .TIMEOUT_TIMEBASE_1_US =
+                                                          d47_get_timer_a_input_clk_TIMEOUT_TIMEBASE_1_US(b)} : d42_get_timer_a_input_clk_tag(b) ==
+        3U ? (t1) {.tag = TAG_ENUM_TIMEOUT_TIMEBASE_1_MS,
+                   .TIMEOUT_TIMEBASE_1_MS =
+                   d46_get_timer_a_input_clk_TIMEOUT_TIMEBASE_1_MS(b)} : d42_get_timer_a_input_clk_tag(b) ==
+        1U ? (t1) {.tag = TAG_ENUM_TIMEOUT_TIMEBASE_10_US,
+                   .TIMEOUT_TIMEBASE_10_US =
+                   d45_get_timer_a_input_clk_TIMEOUT_TIMEBASE_10_US(b)} : (t1) {.tag =
+                                                                                TAG_ENUM_TIMEOUT_TIMEBASE_100_US,
+                                                                                .TIMEOUT_TIMEBASE_100_US =
+                                                                                d44_get_timer_a_input_clk_TIMEOUT_TIMEBASE_100_US(b)};
+}
+static inline unsigned int d50_get_timer_e_input_clk_tag_part0(t3 *b)
+{
+    return (*b).data[0U] >> 8U & 0X7U;
+}
+static inline unsigned int d49_get_timer_e_input_clk_tag(t3 *b)
+{
+    return (unsigned int) d50_get_timer_e_input_clk_tag_part0(b) << 0U;
+}
+static inline unit_t d51_get_timer_e_input_clk_TIMESTAMP_TIMEBASE_100_US(t3 *b)
+{
+    return (unit_t) {.dummy = 0};
+}
+static inline unit_t d52_get_timer_e_input_clk_TIMESTAMP_TIMEBASE_10_US(t3 *b)
+{
+    return (unit_t) {.dummy = 0};
+}
+static inline unit_t d53_get_timer_e_input_clk_TIMESTAMP_TIMEBASE_1_MS(t3 *b)
+{
+    return (unit_t) {.dummy = 0};
+}
+static inline unit_t d54_get_timer_e_input_clk_TIMESTAMP_TIMEBASE_1_US(t3 *b)
+{
+    return (unit_t) {.dummy = 0};
+}
+static inline unit_t d55_get_timer_e_input_clk_TIMESTAMP_TIMEBASE_SYSTEM(t3 *b)
+{
+    return (unit_t) {.dummy = 0};
+}
+static inline t2 d48_get_timer_e_input_clk(t3 *b)
+{
+    return d49_get_timer_e_input_clk_tag(b) == 0U ? (t2) {.tag =
+                                                          TAG_ENUM_TIMESTAMP_TIMEBASE_SYSTEM,
+                                                          .TIMESTAMP_TIMEBASE_SYSTEM =
+                                                          d55_get_timer_e_input_clk_TIMESTAMP_TIMEBASE_SYSTEM(b)} : d49_get_timer_e_input_clk_tag(b) ==
+        1U ? (t2) {.tag = TAG_ENUM_TIMESTAMP_TIMEBASE_1_US,
+                   .TIMESTAMP_TIMEBASE_1_US =
+                   d54_get_timer_e_input_clk_TIMESTAMP_TIMEBASE_1_US(b)} : d49_get_timer_e_input_clk_tag(b) ==
+        4U ? (t2) {.tag = TAG_ENUM_TIMESTAMP_TIMEBASE_1_MS,
+                   .TIMESTAMP_TIMEBASE_1_MS =
+                   d53_get_timer_e_input_clk_TIMESTAMP_TIMEBASE_1_MS(b)} : d49_get_timer_e_input_clk_tag(b) ==
+        2U ? (t2) {.tag = TAG_ENUM_TIMESTAMP_TIMEBASE_10_US,
+                   .TIMESTAMP_TIMEBASE_10_US =
+                   d52_get_timer_e_input_clk_TIMESTAMP_TIMEBASE_10_US(b)} : (t2) {.tag =
+                                                                                  TAG_ENUM_TIMESTAMP_TIMEBASE_100_US,
+                                                                                  .TIMESTAMP_TIMEBASE_100_US =
+                                                                                  d51_get_timer_e_input_clk_TIMESTAMP_TIMEBASE_100_US(b)};
+}
+static inline t3 *reset_timer_e(t3 *a1)
 {
     t3 *r2 = a1;
     u32 r3 = 0U;
@@ -270,27 +270,71 @@ static inline t3 *reset_timer_e_cogent(t3 *a1)
     d4_set_timer_e(r4, r3);
     
     t3 *r5 = r4;
+    u32 r6 = 0U;
+    t3 *r7 = r5;
     
-    return r5;
+    d6_set_timer_e_hi(r7, r6);
+    
+    t3 *r8 = r7;
+    
+    return r8;
 }
-static inline u64 meson_get_time(t6 *a1)
+static inline t8 *initialize(t8 *a1)
 {
-    t6 *r2 = a1;
+    t3 *r2 = (*a1).regs;
+    unit_t r3 = (unit_t) {.dummy = 0};
+    t1 r4;
+    
+    r4 = (t1) {.tag = TAG_ENUM_TIMEOUT_TIMEBASE_1_MS, .TIMEOUT_TIMEBASE_1_MS =
+               r3};
+    
+    t1 r5 = r4;
+    t1 r6 = r5;
+    t3 *r7 = r2;
+    
+    d9_set_timer_a_input_clk(r7, r6);
+    
+    t3 *r8 = r7;
+    unit_t r9 = (unit_t) {.dummy = 0};
+    t2 r10;
+    
+    r10 = (t2) {.tag = TAG_ENUM_TIMESTAMP_TIMEBASE_1_US,
+                .TIMESTAMP_TIMEBASE_1_US = r9};
+    
+    t2 r11 = r10;
+    t2 r12 = r11;
+    t3 *r13 = r8;
+    
+    d16_set_timer_e_input_clk(r13, r12);
+    
+    t3 *r14 = r13;
+    t3 *r15 = reset_timer_e(r14);
+    t8 *r16 = a1;
+    
+    (*r16).regs = r15;
+    
+    t8 *r17 = r16;
+    
+    return r17;
+}
+static inline u64 meson_get_time(t8 *a1)
+{
+    t8 *r2 = a1;
     t3 *r3 = (*r2).regs;
-    u32 r4 = d7_get_timer_e_hi(r3);
+    u32 r4 = d24_get_timer_e_hi(r3);
     u64 r5 = (u64) r4;
     t3 *r6 = (*r2).regs;
-    u32 r7 = d9_get_timer_e(r6);
+    u32 r7 = d26_get_timer_e(r6);
     u64 r8 = (u64) r7;
     t3 *r9 = (*r2).regs;
-    u32 r10 = d7_get_timer_e_hi(r9);
+    u32 r10 = d24_get_timer_e_hi(r9);
     u64 r11 = (u64) r10;
     bool_t r12 = (bool_t) {.boolean = r11 != r5};
     u64 r13;
     
     if (r12.boolean) {
         t3 *r14 = (*r2).regs;
-        u32 r15 = d9_get_timer_e(r14);
+        u32 r15 = d26_get_timer_e(r14);
         u64 r16 = (u64) r15;
         u64 r17 = 32U;
         u64 r18 = r17 >= 64U ? 0U : r11 << r17;
@@ -314,61 +358,21 @@ static inline u64 meson_get_time(t6 *a1)
     
     return r28;
 }
-static inline t6 *meson_init(t11 a1)
+static inline t8 *meson_set_timeout(t28 a1)
 {
-    t6 *r2 = a1.p1;
-    VAddr *r3 = a1.p2;
-    t3 *r4 = config_get_regs(r3);
-    unit_t r5 = (unit_t) {.dummy = 0};
-    t1 r6;
-    
-    r6 = (t1) {.tag = TAG_ENUM_TIMEOUT_TIMEBASE_1_MS, .TIMEOUT_TIMEBASE_1_MS =
-               r5};
-    
-    t1 r7 = r6;
-    t1 r8 = r7;
-    t3 *r9 = r4;
-    
-    d12_set_timer_a_input_clk(r9, r8);
-    
-    t3 *r10 = r9;
-    unit_t r11 = (unit_t) {.dummy = 0};
-    t2 r12;
-    
-    r12 = (t2) {.tag = TAG_ENUM_TIMESTAMP_TIMEBASE_1_US,
-                .TIMESTAMP_TIMEBASE_1_US = r11};
-    
-    t2 r13 = r12;
-    t2 r14 = r13;
-    t3 *r15 = r10;
-    
-    d19_set_timer_e_input_clk(r15, r14);
-    
-    t3 *r16 = r15;
-    t3 *r17 = reset_timer_e(r16);
-    t6 *r18 = r2;
-    
-    (*r18).regs = r17;
-    
-    t6 *r19 = r18;
-    
-    return r19;
-}
-static inline t6 *meson_set_timeout(t27 a1)
-{
-    t6 *r2 = a1.p1;
+    t8 *r2 = a1.p1;
     u16 r3 = a1.p2;
     bool_t r4 = a1.p3;
     t3 *r5 = (*r2).regs;
     t3 *r6 = r5;
     
-    d28_set_timer_a_mode(r6, r4);
+    d29_set_timer_a_mode(r6, r4);
     
     t3 *r7 = r6;
     u32 r8 = (u32) r3;
     t3 *r9 = r7;
     
-    d30_set_timer_a(r9, r8);
+    d31_set_timer_a(r9, r8);
     
     t3 *r10 = r9;
     bool_t r11;
@@ -378,56 +382,56 @@ static inline t6 *meson_set_timeout(t27 a1)
     } else
         ;
     
-    t6 *r12;
+    t8 *r12;
     
     if (r11.boolean) {
         bool_t r13 = (bool_t) {.boolean = 1U};
         t3 *r14 = r10;
         
-        d32_set_timer_a_en(r14, r13);
+        d33_set_timer_a_en(r14, r13);
         
         t3 *r15 = r14;
-        t6 *r16 = r2;
+        t8 *r16 = r2;
         
         (*r16).regs = r15;
         
-        t6 *r17 = r16;
+        t8 *r17 = r16;
         bool_t r18 = (bool_t) {.boolean = 0U};
-        t6 *r19 = r17;
+        t8 *r19 = r17;
         
         (*r19).disable = r18;
         r12 = r19;
     } else {
-        t6 *r20 = r2;
+        t8 *r20 = r2;
         
         (*r20).regs = r10;
         r12 = r20;
     }
     
-    t6 *r21 = r12;
+    t8 *r21 = r12;
     
     return r21;
 }
-static inline t6 *meson_stop_timer(t6 *a1)
+static inline t8 *meson_stop_timer(t8 *a1)
 {
     t3 *r2 = (*a1).regs;
     bool_t r3 = (bool_t) {.boolean = 0U};
     t3 *r4 = r2;
     
-    d32_set_timer_a_en(r4, r3);
+    d33_set_timer_a_en(r4, r3);
     
     t3 *r5 = r4;
-    t6 *r6 = a1;
+    t8 *r6 = a1;
     
     (*r6).regs = r5;
     
-    t6 *r7 = r6;
+    t8 *r7 = r6;
     bool_t r8 = (bool_t) {.boolean = 1U};
-    t6 *r9 = r7;
+    t8 *r9 = r7;
     
     (*r9).disable = r8;
     
-    t6 *r10 = r9;
+    t8 *r10 = r9;
     
     return r10;
 }
