verified_cogent_driver/generated/Driver_CorresProof.thy
@@ -73,9 +73,9 @@ ML \<open>
          verbose;
 \<close>
 ML \<open>
-fun typing_tree_of "reset_timer_e_cogent" = reset_timer_e_cogent_typing_tree
+fun typing_tree_of "reset_timer_e" = reset_timer_e_typing_tree
+  | typing_tree_of "initialize" = initialize_typing_tree
   | typing_tree_of "meson_get_time" = meson_get_time_typing_tree
-  | typing_tree_of "meson_init" = meson_init_typing_tree
   | typing_tree_of "meson_set_timeout" = meson_set_timeout_typing_tree
   | typing_tree_of "meson_stop_timer" = meson_stop_timer_typing_tree
   | typing_tree_of f = error ("No typing tree for " ^ quote f)
@@ -108,7 +108,7 @@ fun name_field ctxt (nm, funcs) = let
 ML \<open>
 val HO_call_hints =
      Cogent_functions
-     |> Par_List.map (fn f => case CogentHigherOrder.make_HO_call_hints @{context} "driver_pp_inferred.c" f of
+     |> Par_List.map (fn f => case CogentHigherOrder.make_HO_call_hints @{context} "driver.c" f of
             [] => [] | hints => [(f, map (name_field @{context}) hints)])
      |> List.concat
      |> Symtab.make
@@ -140,11 +140,11 @@ val Cogent_main_tree =
   |> Symtab.map (K annotate_depth)
 
 val entry_func_names = [
-      "meson_init",
+      "initialize",
       "meson_get_time",
       "meson_set_timeout",
       "meson_stop_timer",
-      "reset_timer_e_cogent"
+      "reset_timer_e"
 ]
 val entry_funcs = Symtab.dest Cogent_main_tree
       |> filter (fn (n, _) => member (op =) entry_func_names n) |> Symtab.make
